CAS new scripting language

cas/theories/Execute.v
@@ -2,44 +2,109 @@ From CAS Require Export
      NetUnix
      Tester.
 From ExtLib Require Export
+     OptionMonad
      Applicative.
 Export
   ApplicativeNotation.
 
-Definition gen_request (ss : server_state exp) : IO (requestT exp) :=
-  io_or
-    (k <- io_choose_ gen_string (map fst ss);;
-     t <- io_choose_ (Exp__Const <$> gen_string) (map (fst ∘ snd) ss);;
-     ret (Request__GET k t))
-    (k <- io_choose_ gen_string (map fst ss);;
-     t <- io_choose_ (Exp__Const <$> gen_string) (map (fst ∘ snd) ss);;
-     Request__CAS k t <$> gen_string).
+Variant texp : Type -> Set :=
+  Texp__FandB : nat -> nat -> texp tag.
 
-Definition fill_tag (tx : exp tag) (es : exp_state) : IO (id tag) :=
-  let gen_tag :=
-      io_choose_ gen_string $
-                 concat (map (fun s =>
-                                match snd s with
-                                | inl t  => [t]
-                                | inr ts => ts
-                                end) es) in
+Definition scriptT : Set := clientT * requestT texp * option (responseT id).
+Definition traceT := list scriptT.
+
+Instance Serialize__texp : Serialize (texp tag) :=
+  fun tx => match tx with
+         | Texp__FandB f b => [Atom "Texp"; to_sexp f; to_sexp b]%sexp
+         end.
+
+Instance Serialize__reqtexp : Serialize (requestT texp) :=
+  fun m =>
+    match m with
+    | Request__GET k t =>
+      [Atom "GET"; to_sexp k; to_sexp t]
+    | Request__CAS k t v =>
+      [Atom "CAS"; to_sexp k; to_sexp t; to_sexp v]
+    end%sexp.
+
+(** Find all [n] s.t. [f (nth n l) = true]. *)
+Definition find_nth' {A} (f : A -> bool) (l : list A) : list (nat * A) :=
+  let index : list nat := seq 0 $ length l in
+  filter (f ∘ snd) $ zip index l.
+
+Definition find_nth {A} (f : A -> bool) : list A -> list nat :=
+  map fst ∘ find_nth' f.
+
+Definition get_tag (sc : scriptT) : option tag :=
+  if snd sc is Some (Response__OK t _) then Some t else None.
+
+Definition has_tag (sc : scriptT) : bool :=
+  if get_tag sc is Some _ then true else false.
+
+Definition arbitraryNat (n : nat) : IO nat :=
+  nat_of_int <$> ORandom.int (int_of_nat n).
+
+Definition arbitraryRequest (ss : server_state exp) (t : traceT)
+  : IO (requestT texp) :=
+  let n :      nat := length           t in
+  let i : list nat := find_nth has_tag t in
+  k <- io_or gen_string (io_choose_ gen_string (map fst ss));;
+  f <- io_choose_ (if n is O then ret O else arbitraryNat n) i;;
+  let t : texp tag := Texp__FandB f (n - S f) in
+  io_or (pure $ Request__GET k t) (Request__CAS k t <$> gen_string).
+
+Definition pick_tag (tr : traceT) : texp tag * tag :=
+  match find_nth' has_tag tr with
+  | [] => (Texp__FandB O O, """Random""")
+  | (f, sc) :: _ =>
+    (Texp__FandB f (length tr - S f),
+     match get_tag sc with
+     | Some t => t
+     | None   => """Random"""    (* should not happen *)
+     end)
+  end.
+
+Definition fill_tag (tr : traceT) (tx : texp tag) : texp tag * id tag :=
+  let n := length tr in
   match tx with
-  | Exp__Const t => io_or (ret t) gen_tag
-  | Exp__Var x =>
-    match get x es with
-    | Some (inl t) => io_or (ret t) gen_tag
-    | Some (inr ts) => io_or (io_choose_ gen_tag ts) gen_tag
-    | None => gen_tag
+  | Texp__FandB f b =>
+    let tf := nth_error tr f        >>= get_tag in
+    let tb := nth_error (rev' tr) b >>= get_tag in
+    match tf, tb with
+    | Some t, _ =>
+      (Texp__FandB f (n - S f), t)
+    | None, Some t =>
+      (Texp__FandB (n - S b) b, t)
+    | None, None => pick_tag tr
     end
-  | Exp__Match _ _ => gen_tag
   end.
 
-Definition fill_request (rx : requestT exp) (es : exp_state)
-  : IO (requestT id) :=
+Definition fill_request (tr : traceT) (rx : requestT texp) : requestT texp * requestT id :=
   match rx with
-  | Request__GET k tx   => Request__GET k <$> fill_tag tx es
-  | Request__CAS k tx v => flip (Request__CAS k) v <$> fill_tag tx es
+  | Request__GET k tx =>
+    let (tx', t) := fill_tag tr tx in
+    (Request__GET k tx', Request__GET k t)
+  | Request__CAS k tx v =>
+    let (tx', t) := fill_tag tr tx in
+    (Request__CAS k tx' v, Request__CAS k t v)
   end.
+
+Definition replace {A} (n : nat) (a : A) (l : list A) : list A :=
+  firstn n l ++ a :: skipn (S n) l.
+
+Definition replace_first {A} (f : A -> bool) (g : A -> A) (l : list A) : list A :=
+  match find_nth' f l with
+  | [] => l
+  | (n, a)::_ => replace n (g a) l
+  end.
+
+Definition fill_trace (c : clientT) (res : responseT id) : traceT -> traceT :=
+  replace_first (fun sc =>
+                let '(c0, _, ores) := sc in
+                if ores is None then c0 =? c else false)%nat
+             (fun sc =>
+                let '(c, req, _) := sc in
+                (c, req, Some res)).
 
 Fixpoint findResponse (s : conn_state)
   : IO (option (packetT id) * conn_state) :=
@@ -58,64 +123,78 @@ Fixpoint findResponse (s : conn_state)
         failwith $ "Bad response " ++ to_string r ++ " received on connection "
                  ++ to_string c
       | inr res =>
-        prerr_endline ("================ RECEIVED =================");;
+        (* prerr_endline ("================ RECEIVED =================");; *)
         let pkt := Packet Conn__Server (Conn__Client c) (inr res) in
-        prerr_endline (to_string pkt);;
+        (* prerr_endline (to_string pkt);; *)
         ret (Some pkt, (c, (f, str')) :: t)
       end
     end
   end.
 
-Fixpoint execute' {R} (fuel : nat) (s : conn_state) (script : list (requestT exp))
-         (m : itree tE R) : IO (bool * conn_state * list (requestT exp)) :=
+Fixpoint execute' {R} (fuel : nat) (s : conn_state) (otrace : option traceT)
+         (acc : traceT) (m : itree tE R)
+  : IO (bool * conn_state * traceT) :=
   match fuel with
-  | O => ret (true, s, [])
+  | O => ret (true, s, acc)
   | S fuel =>
     match observe m with
-    | RetF _ => ret (true, s, [])
-    | TauF m' => execute' fuel s script m'
+    | RetF _ => ret (true, s, acc)
+    | TauF m' => execute' fuel s otrace acc m'
     | VisF e k =>
       match e with
-      | (Throw err|) => ret (false, s, [])
+      | (Throw err|) => ret (false, s, acc)
       | (|ne|) =>
         match ne in nondetE Y return (Y -> _) -> _ with
         | Or => fun k => b <- ORandom.bool tt;;
-                     execute' fuel s script (k b)
+                     execute' fuel s otrace acc (k b)
         end k
       | (||ce) =>
         match ce in clientE Y return (Y -> _) -> _ with
         | Client__Recv =>
           fun k => '(op, s') <- execStateT recv_bytes s >>= findResponse;;
-                execute' fuel s' script (k op)
+                let acc' :=
+                    match op with
+                    | Some (Packet Conn__Server (Conn__Client c) (inr res)) =>
+                      fill_trace c res acc
+                    | _ => acc
+                    end in
+                execute' fuel s' otrace acc' (k op)
         | Client__Send ss es =>
           fun k =>
-            '(sc', rx) <- match script with
-                         | [] => pair [] <$> gen_request ss
-                         | rx :: rs => ret (rs, rx)
-                         end;;
-            req <- fill_request rx es;;
-            '(oc, s1) <- runStateT (send_request req) s;;
-            match oc with
-            | Some c =>
-              prerr_endline ("================== SENT ===================");;
-              let pkt := Packet (Conn__Client c) Conn__Server $ inl req in
-              prerr_endline (to_string pkt);;
-              '(res, s2, tr) <- execute' fuel s1 sc' (k (Some pkt));;
-              ret (res, s2, rx :: tr)
-            | None => execute' fuel s1 sc' (k None)
+            '(orx, ot') <- match otrace with
+                          | Some [] => ret (None, Some [])
+                          | Some (sc :: tr') =>
+                            ret (Some $ snd $ fst sc, Some tr')
+                          | None =>
+                            rx <- arbitraryRequest ss acc;;
+                            ret (Some rx, None)
+                          end;;
+            match orx with
+            | Some rx =>
+              let (rx', req) := fill_request acc rx in
+              '(oc, s1) <- runStateT (send_request req) s;;
+              match oc with
+              | Some c =>
+                (* prerr_endline ("================== SENT ===================");; *)
+                let pkt := Packet (Conn__Client c) Conn__Server $ inl req in
+                (* prerr_endline (to_string pkt);; *)
+                execute' fuel s1 ot' (acc++[(c, rx', None)])%list (k (Some pkt))
+              | None => execute' fuel s1 ot' acc (k None)
+              end
+            | None => execute' fuel s ot' acc (k None)
             end
         end k
       end
     end
   end.
 
-Definition execute {R} (m : itree tE R) (script : list (requestT exp))
-  : IO (bool * list (requestT exp)) :=
-  prerr_endline "<<<<< begin test >>>>>";;
-  '(b, s, ns) <- execute' bigNumber [] [] m;;
-  prerr_endline "<<<<<<< end test >>>>>";;
+Definition execute {R} (m : itree tE R) (otrace : option traceT)
+  : IO (bool * traceT) :=
+  (* prerr_endline "<<<<< begin test >>>>>";; *)
+  '(b, s, t') <- execute' bigNumber [] otrace [] m;;
+  (* prerr_endline "<<<<<<< end test >>>>>";; *)
   fold_left (fun m fd => OUnix.close fd;; m) (map (fst ∘ snd) s) (ret tt);;
-  ret (b, ns).
+  ret (b, t').
 
 Fixpoint shrink_list {A} (l : list A) : list (list A) :=
   match l with
@@ -130,24 +209,33 @@ Fixpoint repeat_list {A} (n : nat) (l : list A) : list A :=
   | S n' => l ++ repeat_list n' l
   end.
 
-Definition shrink_execute' {R} (m : itree tE R) (script : list (requestT exp))
-  : IO (option (list (requestT exp))) :=
+Definition shrink_execute' {R} (m : itree tE R) (trace : traceT)
+  : IO (option traceT) :=
+  prerr_endline "<<<<< begin shrinking >>>>>";;
+  prerr_endline (to_string trace);;
   IO.fix_io
-    (fun shrink_rec ss =>
-       match ss with
+    (fun shrink_rec ts =>
+       match ts with
        | [] => ret None
-       | s :: ss' =>
-         '(b, s') <- execute m s;;
-         if (b : bool) ||| (length script <=? length s')
-         then shrink_rec ss'
-         else ret (Some s')
-       end) (repeat_list 20 $ shrink_list script).
+       | t :: ts' =>
+         '(b, t') <- execute m (Some t);;
+         if (b : bool) ||| (length trace <=? length t')
+         then
+           prerr_endline "<<<<< accepting trace >>>>>";;
+           prerr_endline (to_string t');;
+           shrink_rec ts'
+         else
+           prerr_endline "<<<<< rejecting trace >>>>>";;
+           prerr_endline (to_string t');;
+           prerr_endline "<<<<<<< end shrinking >>>>>";;
+           ret (Some t')
+       end) (repeat_list 20 $ shrink_list trace).
 
 Definition shrink_execute {R} (m : itree tE R) : IO bool :=
-  '(b, s) <- execute m [];;
+  '(b, t) <- execute m None;;
   if b : bool
   then ret true
-  else IO.while_loop (shrink_execute' m) s;; ret false.
+  else IO.while_loop (shrink_execute' m) t;; ret false.
 
 Definition test {R} : itree smE R -> IO bool :=
   shrink_execute ∘ tester ∘ observer _ ∘ compose_switch tcp.
